src/Lustre/Normalization/LNormalization.v
@@ -22,9 +22,9 @@ Module Type LNORMALIZATION
        (Ord : LORDERED Ids Op Syn)
        (Sem : LSEMANTICS Ids Op OpAux Syn Ord CStr)
        (ClSem : LCLOCKSEMANTICS Ids Op OpAux Syn Typ Clo Cau Ord CStr IStr Sem).
-  Declare Module Norm : NORMALIZATION Ids Op OpAux Syn Cau.
+  Declare Module Export Norm : NORMALIZATION Ids Op OpAux Syn Cau.
   Declare Module Export Correct : CORRECTNESS Ids Op OpAux CStr IStr Syn Cau Typ Clo Ord Sem ClSem Norm.
-  Declare Module Idempotence : IDEMPOTENCE Ids Op OpAux Syn Cau Norm.
+  Declare Module Export Idempotence : IDEMPOTENCE Ids Op OpAux Syn Cau Norm.
 End LNORMALIZATION.
 
 Module LNormalizationFun
@@ -41,7 +41,7 @@ Module LNormalizationFun
        (Sem : LSEMANTICS Ids Op OpAux Syn Ord CStr)
        (ClSem : LCLOCKSEMANTICS Ids Op OpAux Syn Typ Clo Cau Ord CStr IStr Sem)
        <: LNORMALIZATION Ids Op OpAux CStr IStr Syn Typ Clo Cau Ord Sem ClSem.
-  Module Norm := NormalizationFun Ids Op OpAux Syn Cau.
+  Module Export Norm := NormalizationFun Ids Op OpAux Syn Cau.
   Module Export Correct := CorrectnessFun Ids Op OpAux CStr IStr Syn Cau Typ Clo Ord Sem ClSem Norm.
-  Module Idempotence := IdempotenceFun Ids Op OpAux Syn Cau Norm.
+  Module Export Idempotence := IdempotenceFun Ids Op OpAux Syn Cau Norm.
 End LNormalizationFun.
